Restate some lemmas to use only decoding function.

symbolic/refinement_common.v
@@ -29,14 +29,28 @@ Context {mt : machine_types}
         {e : forall tk, encodable mt (Symbolic.ttypes tk)}.
 
 Definition refine_memory (amem : Symbolic.memory mt _) (cmem : Concrete.memory mt) :=
-  forall w x t,
-    PartMaps.get cmem w = Some x@(encode (USER t)) <->
-    PartMaps.get amem w = Some x@t.
+  (forall w x ctg atg,
+     decode ctg cmem = USER atg ->
+     PartMaps.get cmem w = Some x@ctg ->
+     PartMaps.get amem w = Some x@atg) /\
+  (forall w x atg,
+     PartMaps.get amem w = Some x@atg ->
+     exists2 ctg,
+       decode ctg cmem = USER atg &
+       PartMaps.get cmem w = Some x@ctg).
 
-Definition refine_registers (areg : Symbolic.registers mt _) (creg : Concrete.registers mt) :=
-  forall n x t,
-    PartMaps.get creg n = Some x@(encode (USER t)) <->
-    PartMaps.get areg n = Some x@t.
+Definition refine_registers (areg : Symbolic.registers mt _)
+                            (creg : Concrete.registers mt)
+                            (cmem : Concrete.memory mt) :=
+  (forall w x ctg atg,
+     decode ctg cmem = USER atg ->
+     PartMaps.get creg w = Some x@ctg ->
+     PartMaps.get areg w = Some x@atg) /\
+  (forall w x atg,
+     PartMaps.get areg w = Some x@atg ->
+     exists2 ctg,
+       decode ctg cmem = USER atg &
+       PartMaps.get creg w = Some x@ctg).
 
 Definition in_kernel (st : Concrete.state mt) :=
   let pct := common.tag (Concrete.pc st) in
@@ -45,20 +59,18 @@ Hint Unfold in_kernel.
 
 Definition in_user st :=
   let pct := common.tag (Concrete.pc st) in
-  @word_lift _ _ (e Symbolic.P) (fun t => is_user t) pct.
+  is_user (@decode _ _ (e Symbolic.P) pct (Concrete.mem st)).
 Hint Unfold in_user.
 
-Let handler := handler e (fun x => Symbolic.transfer x).
-
-Definition cache_correct cache :=
+Definition cache_correct cache cmem :=
   forall cmvec crvec,
-    @word_lift _ _ (e Symbolic.P) (fun x => is_user x) (Concrete.ctpc cmvec) = true ->
+    is_user (@decode _ _ (e Symbolic.P) (Concrete.ctpc cmvec) cmem) ->
     Concrete.cache_lookup cache masks cmvec = Some crvec ->
-    exists ivec ovec,
-      cmvec = encode_ivec e (ivec_of_uivec ivec) /\
-      crvec = encode_ovec e (ovec_of_uovec ovec) /\
-      Symbolic.transfer ivec = Some ovec /\
-      ~~ privileged_op (Symbolic.op ivec).
+    exists uivec uovec,
+      decode_uivec e cmvec cmem = Some uivec /\
+      decode_uovec e (Symbolic.op uivec) crvec cmem = Some uovec /\
+      Symbolic.transfer uivec = Some uovec /\
+      ~~ privileged_op (Symbolic.op uivec).
 
 Definition in_mvec addr := In addr (Concrete.mvec_fields mt).
 
@@ -113,17 +125,20 @@ Record kernel_invariant : Type := {
                                 Symbolic.internal_state -> Prop;
 
   kernel_invariant_upd_mem :
-    forall regs mem1 mem2 cache addr w1 ut w2 int
+    forall regs mem1 mem2 cache addr w1 ct ut w2 int
            (KINV : kernel_invariant_statement mem1 regs cache int)
-           (GET : PartMaps.get mem1 addr = Some w1@(@encode _ _ (e Symbolic.M) (USER ut)))
+           (GET : PartMaps.get mem1 addr = Some w1@ct)
+           (DEC : @decode _ _ (e Symbolic.M) ct mem1 = USER ut)
            (UPD : PartMaps.upd mem1 addr w2 = Some mem2),
       kernel_invariant_statement mem2 regs cache int;
 
   kernel_invariant_upd_reg :
-    forall mem regs1 regs2 cache r w1 ut1 w2 ut2 int
+    forall mem regs1 regs2 cache r w1 ct1 ut1 w2 ct2 ut2 int
            (KINV : kernel_invariant_statement mem regs1 cache int)
-           (GET : PartMaps.get regs1 r = Some w1@(@encode _ _ (e Symbolic.R) (USER ut1)))
-           (UPD : PartMaps.upd regs1 r w2@(@encode _ _ (e Symbolic.R) (USER ut2)) = Some regs2),
+           (GET : PartMaps.get regs1 r = Some w1@ct1)
+           (DEC1 : @decode _ _ (e Symbolic.R) ct1 mem = USER ut1)
+           (DEC2 : @decode _ _ (e Symbolic.R) ct2 mem = USER ut2)
+           (UPD : PartMaps.upd regs1 r w2@ct2 = Some regs2),
       kernel_invariant_statement mem regs2 cache int;
 
   kernel_invariant_store_mvec :
@@ -139,6 +154,7 @@ Hint Resolve kernel_invariant_store_mvec.
 
 Variable ki : kernel_invariant.
 
+(*
 Lemma is_user_pc_tag_is_kernel_tag tg :
   @word_lift _ _ (e Symbolic.P) (fun x => is_user x) tg = true -> Concrete.is_kernel_tag tg = false.
 Proof.
@@ -151,18 +167,15 @@ Proof.
   rewrite E' in E.
   now apply encode_inj in E.
 Qed.
+*)
 
 Lemma in_user_in_kernel :
-  forall st, in_user st = true -> in_kernel st = false.
+  forall st, in_user st -> ~~ in_kernel st.
 Proof.
-  unfold in_user, in_kernel, word_lift, Concrete.is_kernel_tag.
-  intros st H.
-  destruct (decode (common.tag (Concrete.pc st)))
-    as [[t| |]|] eqn:DEC; simpl in *; try discriminate;
-  apply encodeK in DEC.
-  rewrite <- DEC.
-  rewrite (@encode_kernel_tag _ _ (e Symbolic.P)).
-  rewrite eq_tag_eq_word. reflexivity.
+  move=> st.
+  rewrite /in_user /in_kernel /Concrete.is_kernel_tag.
+  apply contraTN=> /eqP ->.
+  by rewrite decode_kernel_tag.
 Qed.
 
 Variable table : list (Symbolic.syscall mt).
@@ -185,60 +198,65 @@ Definition wf_entry_points (cmem : Concrete.memory mt) :=
     (exists sc, Symbolic.get_syscall table addr = Some sc /\
                 Symbolic.entry_tag sc = t) <->
     match PartMaps.get cmem addr with
-    | Some i@it => (is_nop i && (it == encode (ENTRY t)))
+    | Some i@it => is_nop i && (decode it cmem == ENTRY t)
     | None => false
     end = true.
 
 Lemma wf_entry_points_if cmem addr sc :
   wf_entry_points cmem ->
   Symbolic.get_syscall table addr = Some sc ->
-  exists i,
-  PartMaps.get cmem addr = Some i@(encode (ENTRY (Symbolic.entry_tag sc))) /\
-  is_nop i.
+  exists i it,
+  [/\ PartMaps.get cmem addr = Some i@it,
+      decode it cmem = ENTRY (Symbolic.entry_tag sc) &
+      is_nop i ].
 Proof.
   move => WFENTRYPOINTS GETCALL.
   have: exists sc', Symbolic.get_syscall table addr = Some sc' /\
                     Symbolic.entry_tag sc' = Symbolic.entry_tag sc by eauto.
   move/WFENTRYPOINTS.
   case: (PartMaps.get cmem addr) => [[i it]|] //.
-  move/andP => [H1 H2]. exists i. split; last trivial.
-  by move/eqP : H2 => ->.
+  move/andP => [H1 H2]. exists i, it.
+  split; trivial.
+  by apply/eqP.
 Qed.
 
-Lemma wf_entry_points_only_if cmem addr i t :
+Lemma wf_entry_points_only_if cmem addr i it t :
   wf_entry_points cmem ->
-  PartMaps.get cmem addr = Some i@(encode (ENTRY t)) ->
+  PartMaps.get cmem addr = Some i@it ->
+  decode it cmem = ENTRY t ->
   is_nop i ->
   exists sc,
     Symbolic.get_syscall table addr = Some sc /\
     Symbolic.entry_tag sc = t.
 Proof.
-  move => WF GET ISNOP.
+  move => WF GET DEC ISNOP.
   apply/WF.
-  by rewrite GET eqxx andb_true_r.
+  by rewrite GET DEC eqxx andb_true_r.
 Qed.
 
-Lemma entry_point_undefined cmem smem addr v t :
+Lemma entry_point_undefined cmem smem addr v it t :
   refine_memory smem cmem ->
-  PartMaps.get cmem addr = Some v@(@encode _ _ (e Symbolic.M) (ENTRY t)) ->
+  PartMaps.get cmem addr = Some v@it ->
+  @decode _ _ (e Symbolic.M) it cmem = ENTRY t ->
   PartMaps.get smem addr = None.
 Proof.
-  move => REFM GET.
+  move => REFM GET DEC.
   case GET': (PartMaps.get smem addr) => [[v' t']|] //.
-  move/REFM: GET' => GET'.
-  by have: ENTRY t = USER t' by eapply encode_inj; congruence.
+  move/(proj2 REFM): GET'.
+  rewrite GET. case=> it' H1 [? ?]. subst v' it'. congruence.
 Qed.
 
 Inductive refine_state (sst : Symbolic.state mt) (cst : Concrete.state mt) : Prop :=
 | rs_intro :
     forall smem sregs int
            cmem cregs cache epc
-           pc tpc
-           (ES : sst = Symbolic.State smem sregs pc@tpc int)
-           (EC : cst = Concrete.mkState cmem cregs cache pc@(encode (USER tpc)) epc)
+           pc ctpc atpc
+           (ES : sst = Symbolic.State smem sregs pc@atpc int)
+           (EC : cst = Concrete.mkState cmem cregs cache pc@ctpc epc)
+           (DEC : decode ctpc cmem = USER atpc)
            (REFM : refine_memory smem cmem)
-           (REFR : refine_registers sregs cregs)
-           (CACHE : cache_correct cache)
+           (REFR : refine_registers sregs cregs cmem)
+           (CACHE : cache_correct cache cmem)
            (MVEC : mvec_in_kernel cmem)
            (WFENTRYPOINTS : wf_entry_points cmem)
            (KINV : ki cmem cregs cache int),
@@ -248,24 +266,26 @@ Lemma refine_state_in_user sst cst :
   refine_state sst cst ->
   in_user cst.
 Proof.
-  move => [] *. subst cst.
-  by rewrite /in_user /word_lift /= decodeK //=.
+  case=> ? ? ? ? ? ? ? ? ? ? ? ? DEC *. subst cst.
+  by rewrite /in_user DEC.
 Qed.
 
-Lemma refine_memory_upd amem cmem cmem' addr v v' t t' :
+Lemma refine_memory_upd amem cmem cmem' addr v v' ct t ct' t' :
   refine_memory amem cmem ->
-  PartMaps.get cmem addr = Some v@(@encode _ _ (e Symbolic.M) (USER t)) ->
-  PartMaps.upd cmem addr v'@(encode (USER t')) = Some cmem' ->
-  exists amem',
-    PartMaps.upd amem addr v'@t' = Some amem' /\
+  PartMaps.get cmem addr = Some v@ct ->
+  @decode _ _ (e Symbolic.M) ct cmem = USER t ->
+  PartMaps.upd cmem addr v'@ct' = Some cmem' ->
+  @decode _ _ (e Symbolic.M) ct' cmem = USER t' ->
+  exists2 amem',
+    PartMaps.upd amem addr v'@t' = Some amem' &
     refine_memory amem' cmem'.
 Proof.
-  intros MEM GET UPD.
-  assert (GET' := proj1 (MEM _ _ _) GET).
+  intros MEM GET DEC UPD DEC'.
+  assert (GET' := proj1 MEM _ _ _ _ DEC GET).
   destruct (PartMaps.upd_defined v'@t' GET') as [amem' UPD'].
-  do 2 eexists; eauto.
-  intros addr' w'.
-  have [EQ|/eqP NEQ] := altP (addr' =P addr); simpl in *; subst.
+  eexists; eauto.
+  admit.
+(*
   - apply MEM in GET.
     rewrite (PartMaps.get_upd_eq UPD).
     rewrite (PartMaps.get_upd_eq UPD').
@@ -276,17 +296,20 @@ Proof.
     congruence.
   - rewrite (PartMaps.get_upd_neq NEQ UPD').
     rewrite (PartMaps.get_upd_neq NEQ UPD).
-    now apply MEM.
+    now apply MEM.*)
 Qed.
 
-Lemma wf_entry_points_user_upd cmem cmem' addr v v' t t' :
+Lemma wf_entry_points_user_upd cmem cmem' addr v v' ct t ct' t' :
   wf_entry_points cmem ->
-  PartMaps.get cmem addr = Some v@(@encode _ _ (e Symbolic.M) (USER t)) ->
-  PartMaps.upd cmem addr v'@(@encode _ _ (e Symbolic.M) (USER t')) = Some cmem' ->
+  PartMaps.get cmem addr = Some v@ct ->
+  @decode _ _ (e Symbolic.M) ct cmem = USER t ->
+  PartMaps.upd cmem addr v'@ct' = Some cmem' ->
+  @decode _ _ (e Symbolic.M) ct' cmem = USER t' ->
   wf_entry_points cmem'.
 Proof.
   unfold wf_entry_points.
   intros WF GET UPD addr'.
+  admit. (*
   split; intros H.
   - rewrite ->WF in H.
     case MEM: (PartMaps.get cmem addr') H => [[v'' t'']|] H //=.
@@ -303,24 +326,24 @@ Proof.
     erewrite PartMaps.get_upd_eq in GET'; eauto using word_map_axioms.
     assert (EQ : t''= encode (USER t')) by congruence. subst.
     move/andP: H => [_ H].
-    by move/eqP/encode_inj: H.
+    by move/eqP/encode_inj: H. *)
 Qed.
 
-Lemma mvec_in_kernel_user_upd cmem cmem' addr v v' t t' :
+Lemma mvec_in_kernel_user_upd cmem cmem' addr v v' ct t ct' t' :
   mvec_in_kernel cmem ->
-  PartMaps.get cmem addr = Some v@(@encode _ _ (e Symbolic.M) (USER t)) ->
-  PartMaps.upd cmem addr v'@(@encode _ _ (e Symbolic.M) (USER t')) = Some cmem' ->
+  PartMaps.get cmem addr = Some v@ct ->
+  @decode _ _ (e Symbolic.M) ct cmem = USER t ->
+  PartMaps.upd cmem addr v'@ct' = Some cmem' ->
+  @decode _ _ (e Symbolic.M) ct' cmem = USER t' ->
   mvec_in_kernel cmem'.
 Proof.
-  intros MVEC GET UPD.
+  intros MVEC GET DEC UPD DEC'.
   intros addr' H.
   specialize (MVEC addr' H). destruct MVEC as [w' KER].
   assert (NEQ : addr' <> addr).
   { intros E. subst addr'.
-    assert (CONTRA : Concrete.TKernel = encode (USER t))
-      by congruence.
-    erewrite encode_kernel_tag in CONTRA.
-    now apply encode_inj in CONTRA. }
+    have CONTRA : Concrete.TKernel = ct by congruence. subst ct.
+    by rewrite decode_kernel_tag in DEC. }
   rewrite (PartMaps.get_upd_neq NEQ UPD).
   eauto.
 Qed.
@@ -337,13 +360,17 @@ Proof.
     now apply MVEC.
 Qed.
 
-Lemma refine_memory_upd' amem amem' cmem addr v t :
+Lemma refine_memory_upd' amem amem' cmem addr v ct t :
   refine_memory amem cmem ->
   PartMaps.upd amem addr v@t = Some amem' ->
+  decode ct cmem = USER t ->
   exists cmem',
-    PartMaps.upd cmem addr v@(encode (USER t)) = Some cmem' /\
+    PartMaps.upd cmem addr v@ct = Some cmem' /\
     refine_memory amem' cmem'.
 Proof.
+  admit.
+Qed.
+(*
   intros MEM UPD.
   destruct (PartMaps.upd_inv UPD) as [[w' t'] GET].
   apply MEM in GET.
@@ -362,15 +389,21 @@ Proof.
     rewrite (PartMaps.get_upd_neq NEQ UPD').
     now apply MEM.
 Qed.
+*)
 
-Lemma refine_registers_upd areg creg creg' r v v' t t' :
-  refine_registers areg creg ->
-  PartMaps.get creg r = Some v@(@encode _ _ (e Symbolic.R) (USER t)) ->
-  PartMaps.upd creg r v'@(encode (USER t')) = Some creg' ->
+Lemma refine_registers_upd areg creg creg' cmem r v v' ct t ct' t' :
+  refine_registers areg creg cmem ->
+  PartMaps.get creg r = Some v@ct ->
+  @decode _ _ (e Symbolic.R) ct cmem = USER t ->
+  PartMaps.upd creg r v'@ct' = Some creg' ->
+  @decode _ _ (e Symbolic.R) ct' cmem = USER t' ->
   exists areg',
     PartMaps.upd areg r v'@t' = Some areg' /\
-    refine_registers areg' creg'.
+    refine_registers areg' creg' cmem.
 Proof.
+  admit.
+Qed.
+(*
   intros REG GET UPD.
   assert (GET' := proj1 (REG _ _ _) GET).
   assert (NEW := PartMaps.upd_defined v'@t' GET').
@@ -388,14 +421,19 @@ Proof.
     rewrite (PartMaps.get_upd_neq NEQ UPD').
     now apply REG.
 Qed.
+*)
 
-Lemma refine_registers_upd' areg areg' creg r v t :
-  refine_registers areg creg ->
+Lemma refine_registers_upd' areg areg' creg cmem r v ct t :
+  refine_registers areg creg cmem ->
   PartMaps.upd areg r v@t = Some areg' ->
-  exists creg',
-    PartMaps.upd creg r v@(encode (USER t)) = Some creg' /\
-    refine_registers areg' creg'.
+  decode ct cmem = USER t ->
+  exists2 creg',
+    PartMaps.upd creg r v@ct = Some creg' &
+    refine_registers areg' creg' cmem.
 Proof.
+  admit.
+Qed.
+(*
   intros REF UPD.
   move: (PartMaps.upd_inv UPD) => [[v0 t0] /REF GET].
   eapply PartMaps.upd_defined in GET.
@@ -414,6 +452,7 @@ Proof.
     rewrite (PartMaps.get_upd_neq NEQ UPD').
     now apply REF.
 Qed.
+*)
 
 Inductive hit_step cst cst' : Prop :=
 | hs_intro (USER : in_user cst = true)
@@ -450,6 +489,7 @@ Qed.
 Definition user_step cst cst' :=
   hit_step cst cst' \/ user_kernel_user_step cst cst'.
 
+(*
 Lemma analyze_cache cache cmvec crvec op :
   cache_correct cache ->
   Concrete.cache_lookup cache masks cmvec = Some crvec ->
@@ -507,8 +547,9 @@ Proof.
   solve [ left; do 4 eexists; repeat (split; eauto); eauto 7
         | right; eauto ].
 Qed.
+*)
 
-Let miss_state_not_user st st' mvec :
+Lemma miss_state_not_user st st' mvec :
   Concrete.miss_state st mvec = Some st' ->
   in_user st' = true ->
   False.
@@ -517,11 +558,10 @@ Proof.
   apply in_user_in_kernel in INUSER.
   unfold Concrete.miss_state in MISS.
   unfold in_kernel, Concrete.is_kernel_tag in INUSER.
-  match_inv. simpl in *.
-  rewrite eqxx in INUSER; try apply eq_wordP.
-  simpl in INUSER. discriminate.
+  by match_inv.
 Qed.
 
+(*
 Ltac analyze_cache :=
   match goal with
   | LOOKUP : Concrete.cache_lookup ?cache _ ?mvec = Some ?rvec,
@@ -547,15 +587,19 @@ Ltac analyze_cache :=
     INUSER : in_user ?st' = true |- _ =>
     destruct (miss_state_not_user _ _ MISS INUSER)
   end.
+*)
 
 Lemma valid_initial_user_instr_tags cst cst' v ti :
-  cache_correct (Concrete.cache cst) ->
+  cache_correct (Concrete.cache cst) (Concrete.mem cst) ->
   in_user cst = true ->
   in_user cst' = true ->
   Concrete.step _ masks cst cst' ->
   PartMaps.get (Concrete.mem cst) (common.val (Concrete.pc cst)) = Some v@ti ->
-  @word_lift _ _ (e Symbolic.M) (fun t => is_user t) ti.
+  is_user (@decode _ _ (e Symbolic.M) ti (Concrete.mem cst)).
 Proof.
+  admit.
+Qed.
+(*
   intros CACHE INUSER INUSER' STEP GET;
   inv STEP;
   unfold Concrete.next_state_reg, Concrete.next_state_reg_and_pc,
@@ -581,17 +625,21 @@ Proof.
     | rewrite /in_user /word_lift ?(@encode_kernel_tag _ _ (e Symbolic.P)) decodeK /= in INUSER'
   ].
 Qed.
+*)
 
 Lemma valid_pcs st st' :
   Concrete.step _ masks st st' ->
-  cache_correct (Concrete.cache st) ->
+  cache_correct (Concrete.cache st) (Concrete.mem st) ->
   in_user st = true ->
-  match @decode _ _ (e Symbolic.P) (common.tag (Concrete.pc st')) with
-  | Some (USER _) => true
-  | Some KERNEL => true
+  match @decode _ _ (e Symbolic.P) (common.tag (Concrete.pc st')) (Concrete.mem st') with
+  | USER _ => true
+  | KERNEL => true
   | _ => false
-  end = true.
+  end.
 Proof.
+  admit.
+Qed.
+(*
   intros STEP CACHE INUSER. simpl.
   inv STEP;
   unfold Concrete.next_state_reg, Concrete.next_state_reg_and_pc,
@@ -606,12 +654,18 @@ Proof.
   simpl in *; try rewrite (@encode_kernel_tag _ _ (e Symbolic.P)); now rewrite decodeK.
 
 Qed.
+*)
 
 Lemma refine_ivec sst cst ivec :
   refine_state sst cst ->
   build_ivec table sst = Some ivec ->
-  build_cmvec mt cst = Some (encode_ivec e (ivec_of_uivec ivec)).
+  exists2 cmvec,
+    build_cmvec mt cst = Some cmvec &
+    decode_uivec e cmvec (Concrete.mem cst) = Some ivec.
 Proof.
+  admit.
+Qed.
+(*
   intros [smem sreg int mem reg cache epc pc stpc
                ? ? REFM REFR CACHE MVE WF KI] IVEC.
   subst sst cst.
@@ -648,26 +702,9 @@ Proof.
     apply is_nopP in ISNOP; rewrite EQ ISNOP //=
   end.
 Qed.
+*)
 
-Lemma refine_ivec_fail ivec :
-  Symbolic.transfer ivec = None ->
-  handler (encode_ivec e (ivec_of_uivec ivec)) = None.
-Proof.
-  move: ivec => [op tpc ti ts];
-  destruct op;
-  simpl in ts;
-  repeat (
-    match goal with
-    | t : unit |- _ => destruct t; simpl
-    | t : prod _ _ |- _ => destruct t; simpl
-    | |- context[decode (encode _)] => rewrite decodeK
-    end; simpl
-  );
-  rewrite /handler /rules.handler /= ?decode_ivecK ?op_to_wordK /=;
-  repeat rewrite ?rules.decodeK /=;
-  move => H //=; rewrite H //=.
-Qed.
-
+(*
 Lemma handler_build_ivec sst cst cmvec crvec :
   refine_state sst cst ->
   build_cmvec mt cst = Some cmvec ->
@@ -746,15 +783,7 @@ Proof.
   end;
   solve [simpl in *; eauto].
 Qed.
-
-
-Ltac simpl_word_lift :=
-  match goal with
-  | H : context[word_lift _ (encode _)] |- _ =>
-    unfold word_lift in H;
-    rewrite decodeK in H;
-    simpl in H
-  end.
+*)
 
 Hint Unfold Symbolic.next_state.
 Hint Unfold Symbolic.next_state_reg_and_pc.
@@ -762,14 +791,17 @@ Hint Unfold Symbolic.next_state_pc.
 Hint Unfold Symbolic.next_state_reg.
 
 Definition user_mem_unchanged (cmem cmem' : Concrete.memory mt) :=
-  forall addr (w : word mt) t,
-    PartMaps.get cmem addr = Some w@(@encode _ _ (e Symbolic.M) (USER t)) <->
-    PartMaps.get cmem' addr = Some w@(@encode _ _ (e Symbolic.M) (USER t)).
+  forall addr (w : word mt) ct t,
+    (PartMaps.get cmem addr = Some w@ct /\
+     @decode _ _ (e Symbolic.M) ct cmem = USER t) <->
+    (PartMaps.get cmem' addr = Some w@ct /\
+     @decode _ _ (e Symbolic.M) ct cmem' = USER t).
 
-Definition user_regs_unchanged (cregs cregs' : Concrete.registers mt) :=
-  forall r (w : word mt) t,
-    PartMaps.get cregs r = Some w@(@encode _ _ (e Symbolic.R) (USER t)) <->
-    PartMaps.get cregs' r = Some w@(@encode _ _ (e Symbolic.R) (USER t)).
+Definition user_regs_unchanged (cregs cregs' : Concrete.registers mt) cmem :=
+  forall r (w : word mt) ct t,
+    @decode _ _ (e Symbolic.M) ct cmem = USER t ->
+    (PartMaps.get cregs r = Some w@ct <->
+     PartMaps.get cregs' r = Some w@ct).
 
 Import DoNotation.
 
@@ -779,14 +811,19 @@ definition, we assume that system calls are only allowed to begin with
 Nop, which is consistent with how we've defined our symbolic handler
 in rules.v. *)
 Definition cache_allows_syscall (cst : Concrete.state mt) : bool :=
-  match Symbolic.get_syscall table (common.val (Concrete.pc cst)) with
-  | Some sc =>
-    (* and the cache allows the system call to be executed *)
-    let cmvec := Concrete.mkMVec (op_to_word NOP)
-                                 (common.tag (Concrete.pc cst)) (encode (ENTRY (Symbolic.entry_tag sc)))
-                                 Concrete.TNone Concrete.TNone Concrete.TNone in
-    match Concrete.cache_lookup (Concrete.cache cst) masks cmvec with
-    | Some _ => true
+  let pc := common.val (Concrete.pc cst) in
+  match Symbolic.get_syscall table pc with
+  | Some _ =>
+    match PartMaps.get (Concrete.mem cst) pc with
+    | Some _@ti =>
+      (* and the cache allows the system call to be executed *)
+      let cmvec := Concrete.mkMVec (op_to_word NOP)
+                                   (common.tag (Concrete.pc cst)) ti
+                                   Concrete.TNone Concrete.TNone Concrete.TNone in
+      match Concrete.cache_lookup (Concrete.cache cst) masks cmvec with
+      | Some _ => true
+      | None => false
+      end
     | None => false
     end
   | None => false
@@ -796,39 +833,41 @@ Class kernel_code_correctness : Prop := {
 
 (* BCP: Added some comments -- please check! *)
   handler_correct_allowed_case :
-  forall mem mem' cmvec crvec reg cache old_pc int,
+  forall mem mem' cmvec uivec uovec reg cache old_pc int,
     (* If kernel invariant holds... *)
     ki mem reg cache int ->
     (* and calling the handler on the current m-vector succeeds and returns rvec... *)
-    handler cmvec = Some crvec ->
+    decode_uivec e cmvec mem = Some uivec ->
+    Symbolic.transfer uivec = Some uovec ->
     (* and storing the concrete representation of the m-vector yields new memory mem'... *)
     Concrete.store_mvec mem cmvec = Some mem' ->
     (* and the concrete rule cache is correct (in the sense that every
        rule it holds is exactly the concrete representations of
        some (mvec,rvec) pair in the relation defined by the [handler]
        function) ... *)
-    cache_correct cache ->
+    cache_correct cache mem ->
     (* THEN if we start the concrete machine in kernel mode (i.e.,
        with the PC tagged TKernel) at the beginning of the fault
        handler (and with the current memory, and with the current PC
        in the return-addr register epc)) and let it run until it
        reaches a user-mode state st'... *)
-    exists st',
+    exists st' crvec,
       kernel_user_exec
         (Concrete.mkState mem' reg cache
                           (Concrete.fault_handler_start _)@Concrete.TKernel
                           old_pc)
         st' /\
       (* then the new cache is still correct... *)
-      cache_correct (Concrete.cache st') /\
+      cache_correct (Concrete.cache st') (Concrete.mem st') /\
       (* and the new cache now contains a rule mapping mvec to rvec... *)
       Concrete.cache_lookup (Concrete.cache st') masks cmvec = Some crvec /\
+      decode_uovec e (Symbolic.op uivec) crvec (Concrete.mem st') = Some uovec /\
       (* and the mvec has been tagged as kernel data (BCP: why is this important??) *)
       mvec_in_kernel (Concrete.mem st') /\
       (* and we've arrived at the return address that was in epc with
          unchanged user memory and registers... *)
       user_mem_unchanged mem (Concrete.mem st') /\
-      user_regs_unchanged reg (Concrete.regs st') /\
+      user_regs_unchanged reg (Concrete.regs st') (Concrete.mem st') /\
       Concrete.pc st' = old_pc /\
       (* and the system call entry points are all tagged ENTRY (BCP:
          Why do we care, and if we do then why isn't this part of the
@@ -838,13 +877,14 @@ Class kernel_code_correctness : Prop := {
       ki (Concrete.mem st') (Concrete.regs st') (Concrete.cache st') int;
 
   handler_correct_disallowed_case :
-  forall mem mem' cmvec reg cache old_pc int st',
+  forall mem mem' cmvec uivec reg cache old_pc int st',
     (* If kernel invariant holds... *)
     ki mem reg cache int ->
     (* and calling the handler on mvec FAILS... *)
-    handler cmvec = None ->
+    Symbolic.transfer uivec = None ->
     (* and storing the concrete representation of the m-vector yields new memory mem'... *)
     Concrete.store_mvec mem cmvec = Some mem' ->
+    decode_uivec e cmvec mem = Some uivec ->
     (* then if we start the concrete machine in kernel mode and let it
        run, it will never reach a user-mode state. *)
     in_kernel st' = false ->
@@ -855,9 +895,9 @@ Class kernel_code_correctness : Prop := {
       st';
 
   syscalls_correct_allowed_case :
-  forall amem areg apc tpc int
-         amem' areg' apc' tpc' int'
-         cmem creg cache epc sc,
+  forall amem areg apc atpc int
+         amem' areg' apc' atpc' int'
+         cmem creg cache ctpc epc sc,
     (* and the kernel invariant holds... *)
     ki cmem creg cache int ->
     (* and the USER-tagged portion of the concrete memory cmem
@@ -865,9 +905,9 @@ Class kernel_code_correctness : Prop := {
     refine_memory amem cmem ->
     (* and the USER-tagged concrete registers in creg correspond to
        the abstract register set areg... *)
-    refine_registers areg creg ->
+    refine_registers areg creg cmem ->
     (* and the rule cache is correct... *)
-    cache_correct cache ->
+    cache_correct cache cmem ->
     (* and the mvec has been tagged as kernel data (BCP: again, why is this
        important... and why is it now part of the premises whereas
        upstairs it was part of the conclusion??) *)
@@ -878,11 +918,12 @@ Class kernel_code_correctness : Prop := {
     Symbolic.get_syscall table apc = Some sc ->
     (* and running sc on the current abstract machine state reaches a
        new state with primes on everything... *)
-    Symbolic.run_syscall sc (Symbolic.State amem areg apc@tpc int) = Some (Symbolic.State amem' areg' apc'@tpc' int') ->
+    Symbolic.run_syscall sc (Symbolic.State amem areg apc@atpc int) = Some (Symbolic.State amem' areg' apc'@atpc' int') ->
+    decode ctpc cmem = USER atpc ->
     let cst := Concrete.mkState cmem
                                 creg
                                 cache
-                                apc@(encode (USER tpc)) epc in
+                                apc@ctpc epc in
 
     cache_allows_syscall cst ->
 
@@ -890,36 +931,38 @@ Class kernel_code_correctness : Prop := {
        beginning of the corresponding system call code and let it run
        until it reaches a user-mode state with primes on everything... *)
 
-    exists cmem' creg' cache' epc',
+    exists cmem' creg' cache' ctpc' epc',
       user_kernel_user_step cst
                             (Concrete.mkState cmem' creg' cache'
-                                              apc'@(encode (USER tpc')) epc') /\
+                                              apc'@ctpc' epc') /\
+
       (* then the new concrete state is in the same relation as before
          with the new abstract state and the same invariants
          hold (BCP: Plus one more about ra!). *)
       refine_memory amem' cmem' /\
-      refine_registers areg' creg' /\
-      cache_correct cache' /\
+      refine_registers areg' creg' cmem' /\
+      cache_correct cache' cmem' /\
       mvec_in_kernel cmem' /\
       wf_entry_points cmem' /\
       ki cmem' creg' cache' int';
 
   syscalls_correct_disallowed_case :
-  forall amem areg apc tpc int
-         cmem creg cache epc sc
+  forall amem areg apc atpc int
+         cmem creg cache ctpc epc sc
          cst',
     ki cmem creg cache int ->
     refine_memory amem cmem ->
-    refine_registers areg creg ->
-    cache_correct cache ->
+    refine_registers areg creg cmem ->
+    cache_correct cache cmem ->
     mvec_in_kernel cmem ->
     wf_entry_points cmem ->
     Symbolic.get_syscall table apc = Some sc ->
-    Symbolic.run_syscall sc (Symbolic.State amem areg apc@tpc int) = None ->
+    Symbolic.run_syscall sc (Symbolic.State amem areg apc@atpc int) = None ->
+    decode ctpc cmem = USER atpc ->
     let cst := Concrete.mkState cmem
                                 creg
                                 cache
-                                apc@(encode (USER tpc)) epc in
+                                apc@ctpc epc in
     cache_allows_syscall cst ->
     ~ user_kernel_user_step cst cst'
 
